example/Fibonacci.thy
@@ -1,5 +1,5 @@
 theory Fibonacci
-  imports "../DP_Lifting" "../DP_Consistency"
+  imports "../DP_Lifting" "../DP_Consistency" "../DP_Proof"
 begin
   
   (*
@@ -14,12 +14,12 @@ fun fib :: "nat \<Rightarrow> int option" where
   "fib 0 = Some 0"
 | "fib (Suc 0) = Some 1"
 | "fib (Suc (Suc n)) = case_prod
-      (\<lambda>of1. (\<lambda>of0. case_option
+      (\<lambda>of1 of0. case_option
         None
         (\<lambda>f1. case_option
           None
           (\<lambda>f0. Some (f1 + f0))
-          of0))
+          of0)
         of1)
       (Pair (fib (Suc n)) (fib n))"
 thm fib.simps
@@ -28,24 +28,19 @@ term 0 (**)
 fun fib\<^sub>T :: "nat \<Rightarrow>\<^sub>T int option" where
   "fib\<^sub>T$ 0 =CHECKMEM= \<langle>Some 0\<rangle>"
 | "fib\<^sub>T$ (Suc 0) =CHECKMEM= \<langle>Some 1\<rangle>"
-| "fib\<^sub>T$ (Suc (Suc n)) =CHECKMEM= \<langle>case_prod\<^sub>T\<rangle>
-    . \<langle>\<lambda>of1. \<langle>\<lambda>of0. \<langle>case_option\<^sub>T\<rangle>
+| "fib\<^sub>T$ (Suc (Suc n)) =CHECKMEM= case_prod\<^sub>T
+    . (\<lambda>\<^sub>T of1 of0. case_option\<^sub>T
         . \<langle>None\<rangle>
-        . \<langle>\<lambda>f1. \<langle>case_option\<^sub>T\<rangle>
+        . (\<lambda>\<^sub>T f1. case_option\<^sub>T
           . \<langle>None\<rangle>
-          . \<langle>\<lambda>f0. \<langle>Some (f1 + f0)\<rangle>\<rangle>
-          . \<langle>of0\<rangle>\<rangle>\<rangle>
-        . \<langle>of1\<rangle>\<rangle>
-    . (\<langle>Pair\<^sub>T\<rangle> . (fib\<^sub>T (Suc n)) . (fib\<^sub>T n))"
+          . (\<lambda>\<^sub>T f0. \<langle>Some (f1 + f0)\<rangle>)
+          . \<langle>of0\<rangle>)
+        . \<langle>of1\<rangle>)
+    . (Pair\<^sub>T . (fib\<^sub>T (Suc n)) . (fib\<^sub>T n))"
 term 0 (**)
 
 interpretation fib: dp_consistency fib .
 
 lemma "fib.consistentDP fib\<^sub>T"
-  apply (rule fib.consistentDP_intro, induct_tac rule: fib\<^sub>T.induct, unfold fib\<^sub>T.simps; rule fib.consistentS_checkmem, unfold fib.simps)
-  subgoal premises [transfer_rule] by transfer_prover
-  subgoal premises [transfer_rule] by transfer_prover
-  subgoal premises [transfer_rule] by transfer_prover
-  done
-
+  by (dp_match induct: fib\<^sub>T.induct simp: fib.simps simp\<^sub>T: fib\<^sub>T.simps)
 end
