DP_Consistency.thy
@@ -102,12 +102,8 @@ lemma bind_transfer[transfer_rule]:
   unfolding bind_def rel_fun_def by (fastforce intro: consistentS_intro elim: consistentS_elim split: prod.split)
     
 lemma fun_app_lifted_transfer[transfer_rule]:
-  "(consistentS (R0 ===>\<^sub>T R1) ===> consistentS R0 ===> consistentS R1) (op .) (op .\<^sub>T)"
+  "(consistentS (R0 ===>\<^sub>T R1) ===> consistentS R0 ===> consistentS R1) (\<lambda> f x. f x) (op .)"
   unfolding fun_app_def fun_app_lifted_def by transfer_prover
-
-lemma fun_app_lifted_transfer':
-  "(consistentS (R0 ===>\<^sub>T R1) ===> consistentS R0 ===> consistentS R1) (\<lambda> f x. f x) (op .\<^sub>T)"
-  unfolding fun_app_lifted_def by transfer_prover
 
 term 0 (**)
 
@@ -118,105 +114,117 @@ term 0 (**)
   
 lemma unlift_3_transfer[transfer_rule]:
   "((R0 ===>\<^sub>T R1) ===> (R0 ===> consistentS R1)) (\<lambda> f x. f x) unlift_3"
-  unfolding unlift_3_def supply [transfer_rule] = fun_app_lifted_transfer' by transfer_prover
+  unfolding unlift_3_def by transfer_prover
 term 0 (**)
   
 lemma unlift_33_transfer[transfer_rule]:
   "((R0 ===>\<^sub>T R1 ===>\<^sub>T R2) ===> (R0 ===> R1 ===> consistentS R2)) (\<lambda> f x0 x1. f x0 x1) unlift_33"
-  unfolding unlift_33_def supply [transfer_rule] = fun_app_lifted_transfer' by transfer_prover
+  unfolding unlift_33_def by transfer_prover
 
 lemma lift_'_transfer[transfer_rule]:
-  "(R ===> R) (\<lambda> x. x) lift_'"
+  "(R ===> consistentS R) (\<lambda> x. x) lift_'"
   unfolding lift_'_def by transfer_prover
 
 lemma lift_3_transfer[transfer_rule]:
-  "((R0 ===> R1) ===> (R0 ===>\<^sub>T R1)) (\<lambda> f x. f x) lift_3"
+  "((R0 ===> R1) ===> consistentS (R0 ===>\<^sub>T R1)) (\<lambda> f x. f x) lift_3"
   unfolding lift_3_def by transfer_prover
     
 lemma lift_33_transfer[transfer_rule]:
-  "((R0 ===> R1 ===> R2) ===> (R0 ===>\<^sub>T R1 ===>\<^sub>T R2)) (\<lambda> f x0 x1. f x0 x1) lift_33"
+  "((R0 ===> R1 ===> R2) ===> consistentS (R0 ===>\<^sub>T R1 ===>\<^sub>T R2)) (\<lambda> f x0 x1. f x0 x1) lift_33"
   unfolding lift_33_def by transfer_prover
 
 lemma lift_333_transfer[transfer_rule]:
-  "((R0 ===> R1 ===> R2 ===> R3) ===> (R0 ===>\<^sub>T R1 ===>\<^sub>T R2 ===>\<^sub>T R3)) (\<lambda> f x0 x1 x2. f x0 x1 x2) lift_333"
+  "((R0 ===> R1 ===> R2 ===> R3) ===> consistentS (R0 ===>\<^sub>T R1 ===>\<^sub>T R2 ===>\<^sub>T R3)) (\<lambda> f x0 x1 x2. f x0 x1 x2) lift_333"
   unfolding lift_333_def by transfer_prover
+term 0 (**)
 
+lemma If_transfer[transfer_rule]:
+  "consistentS (op = ===>\<^sub>T R ===>\<^sub>T R ===>\<^sub>T R) If If\<^sub>T"
+  unfolding If\<^sub>T_def by transfer_prover
 term 0 (**)
   
 lemma case_option_transfer[transfer_rule]:
-  "(R1 ===>\<^sub>T (R0 ===>\<^sub>T R1) ===>\<^sub>T rel_option R0 ===>\<^sub>T R1) case_option case_option\<^sub>T"
-  unfolding case_option\<^sub>T_def supply [transfer_rule] = fun_app_lifted_transfer' by transfer_prover
+  "consistentS (R1 ===>\<^sub>T (R0 ===>\<^sub>T R1) ===>\<^sub>T rel_option R0 ===>\<^sub>T R1) case_option case_option\<^sub>T"
+  unfolding case_option\<^sub>T_def by transfer_prover
     
 term 0 (**)
   
 lemma case_list_transfer[transfer_rule]:
-  "(R1 ===>\<^sub>T (R0 ===>\<^sub>T list_all2 R0 ===>\<^sub>T R1) ===>\<^sub>T list_all2 R0 ===>\<^sub>T R1) case_list case_list\<^sub>T"
+  "consistentS (R1 ===>\<^sub>T (R0 ===>\<^sub>T list_all2 R0 ===>\<^sub>T R1) ===>\<^sub>T list_all2 R0 ===>\<^sub>T R1) case_list case_list\<^sub>T"
   unfolding case_list\<^sub>T_def by transfer_prover
 term 0 (**)
   
 lemma case_prod_transfer[transfer_rule]:
-  "((R0 ===>\<^sub>T R1 ===>\<^sub>T R2) ===>\<^sub>T rel_prod R0 R1 ===>\<^sub>T R2) case_prod case_prod\<^sub>T"
+  "consistentS ((R0 ===>\<^sub>T R1 ===>\<^sub>T R2) ===>\<^sub>T rel_prod R0 R1 ===>\<^sub>T R2) case_prod case_prod\<^sub>T"
   unfolding case_prod\<^sub>T_def by transfer_prover
 term 0 (**)
   
 term 0 (**)
 lemma id_transfer[transfer_rule]:
-  "(R ===>\<^sub>T R) id id\<^sub>T"
+  "consistentS (R ===>\<^sub>T R) id id\<^sub>T"
   unfolding id_def id\<^sub>T_def by transfer_prover
 term 0 (**)
   
 lemma plus_transfer[transfer_rule]:
-  "(op = ===>\<^sub>T op = ===>\<^sub>T op =) plus plus\<^sub>T"
+  "consistentS (op = ===>\<^sub>T op = ===>\<^sub>T op =) plus plus\<^sub>T"
   unfolding plus\<^sub>T_def by transfer_prover
 term 0 (**)
   
 lemma Cons_transfer[transfer_rule]:
-  "(R ===>\<^sub>T list_all2 R ===>\<^sub>T list_all2 R) Cons Cons\<^sub>T"
+  "consistentS (R ===>\<^sub>T list_all2 R ===>\<^sub>T list_all2 R) Cons Cons\<^sub>T"
   unfolding Cons\<^sub>T_def by transfer_prover
 term 0 (**)
   
 lemma Some_transfer[transfer_rule]:
-  "(R ===>\<^sub>T rel_option R) Some Some\<^sub>T"
+  "consistentS (R ===>\<^sub>T rel_option R) Some Some\<^sub>T"
   unfolding Some\<^sub>T_def by transfer_prover
 term 0 (**)
   
 lemma Pair_transfer[transfer_rule]:
-  "(R0 ===>\<^sub>T R1 ===>\<^sub>T rel_prod R0 R1) Pair Pair\<^sub>T"
+  "consistentS (R0 ===>\<^sub>T R1 ===>\<^sub>T rel_prod R0 R1) Pair Pair\<^sub>T"
   unfolding Pair\<^sub>T_def by transfer_prover
 term 0 (**)
   
 lemma min_transfer[transfer_rule]:
-  "(op = ===>\<^sub>T op = ===>\<^sub>T op =) min min\<^sub>T"
+  "consistentS (op = ===>\<^sub>T op = ===>\<^sub>T op =) min min\<^sub>T"
   unfolding min\<^sub>T_def by transfer_prover
     
+lemma max_transfer[transfer_rule]:
+  "consistentS (op = ===>\<^sub>T op = ===>\<^sub>T op =) max max\<^sub>T"
+  unfolding max\<^sub>T_def by transfer_prover
+    
 lemma upt_transfer[transfer_rule]:
-  "(op = ===>\<^sub>T op = ===>\<^sub>T list_all2 op =) upt upt\<^sub>T"
+  "consistentS (op = ===>\<^sub>T op = ===>\<^sub>T list_all2 op =) upt upt\<^sub>T"
   unfolding upt\<^sub>T_def by transfer_prover
     
 lemma comp_transfer[transfer_rule]:
-  "((R1 ===>\<^sub>T R2) ===>\<^sub>T (R0 ===>\<^sub>T R1) ===>\<^sub>T (R0 ===>\<^sub>T R2)) comp comp\<^sub>T"
+  "consistentS ((R1 ===>\<^sub>T R2) ===>\<^sub>T (R0 ===>\<^sub>T R1) ===>\<^sub>T (R0 ===>\<^sub>T R2)) comp comp\<^sub>T"
   unfolding comp_def comp\<^sub>T_def fun_app_lifted_def by transfer_prover
     
 lemma map_transfer[transfer_rule]:
-  "((R0 ===>\<^sub>T R1) ===>\<^sub>T list_all2 R0 ===>\<^sub>T list_all2 R1) map map\<^sub>T"
-  apply (unfold map\<^sub>T_def, rule rel_funI, rule return_transfer[THEN rel_funD], rule rel_funI)
-  apply (induct_tac rule: list_all2_induct, assumption; unfold list.map map\<^sub>T'.simps fun_app_lifted_def)
-  subgoal premises [transfer_rule] by transfer_prover
-  subgoal premises [transfer_rule] by transfer_prover
-  done
-term 0 (**)
+  "consistentS ((R0 ===>\<^sub>T R1) ===>\<^sub>T list_all2 R0 ===>\<^sub>T list_all2 R1) map map\<^sub>T"
+proof -
+  have [transfer_rule]: "((R0 ===>\<^sub>T R1) ===> (list_all2 R0 ===>\<^sub>T list_all2 R1)) map map\<^sub>T'"
+    apply ((rule rel_funI)+, induct_tac rule: list_all2_induct, assumption; unfold list.map map\<^sub>T'.simps)
+    subgoal premises [transfer_rule] by transfer_prover
+    subgoal premises [transfer_rule] by transfer_prover
+    done
+  show ?thesis
+    unfolding map\<^sub>T_def by transfer_prover
+qed
   
 lemma fold_transfer[transfer_rule]:
-  "((R0 ===>\<^sub>T R1 ===>\<^sub>T R1) ===>\<^sub>T list_all2 R0 ===>\<^sub>T R1 ===>\<^sub>T R1) fold fold\<^sub>T"
-  apply (unfold fold\<^sub>T_def, rule rel_funI, rule return_transfer[THEN rel_funD], rule rel_funI)
-  apply (induct_tac rule: list_all2_induct, assumption; unfold fold.simps fold\<^sub>T'.simps fun_app_lifted_def)
-  subgoal premises [transfer_rule] by transfer_prover
-  subgoal premises [transfer_rule] by transfer_prover
-  done
+  "consistentS ((R0 ===>\<^sub>T R1 ===>\<^sub>T R1) ===>\<^sub>T list_all2 R0 ===>\<^sub>T R1 ===>\<^sub>T R1) fold fold\<^sub>T"
+proof -
+  have [transfer_rule]: "((R0 ===>\<^sub>T R1 ===>\<^sub>T R1) ===> list_all2 R0 ===>\<^sub>T R1 ===>\<^sub>T R1) fold fold\<^sub>T'"
+    apply ((rule rel_funI)+, induct_tac rule: list_all2_induct, assumption; unfold fold.simps fold\<^sub>T'.simps)
+    subgoal premises [transfer_rule] by transfer_prover
+    subgoal premises [transfer_rule] by transfer_prover
+    done
+  show ?thesis
+    unfolding fold\<^sub>T_def by transfer_prover
+qed
 
 end
 end
-
-notation dp_consistency.rel_fun_lifted (infixr "===>\<^sub>T" 55)
-
 end
