example/Knapsack.thy
@@ -1,0 +1,26 @@
+theory Knapsack
+  imports "../DP_Consistency" "../DP_Proof"
+begin
+context (* Knapsack *)
+  fixes w :: "nat \<Rightarrow> nat"
+begin
+  
+fun su :: "nat\<times>nat \<Rightarrow> nat" where
+  "su (0, W) = (if W < w 0 then 0 else w 0)" |
+  "su (Suc i, W) = (if W < w (Suc i)
+    then su (i, W)
+    else max (su (i, W)) (w i + su (i, W - w i)))"
+  
+fun su\<^sub>T :: "nat\<times>nat \<Rightarrow>\<^sub>T nat" where
+  "su\<^sub>T$ (0, W) =CHECKMEM= If\<^sub>T . \<langle>W < w 0\<rangle> . \<langle>0\<rangle> . \<langle>w 0\<rangle>" |
+  "su\<^sub>T$ (Suc i, W) =CHECKMEM= If\<^sub>T . \<langle>W < w (Suc i)\<rangle>
+    . (su\<^sub>T (i, W))
+    . (max\<^sub>T . (su\<^sub>T (i, W)) . (plus\<^sub>T . \<langle>w i\<rangle> . (su\<^sub>T (i, W - w i))))"
+
+interpretation su: dp_consistency su .
+
+lemma "su.consistentDP su\<^sub>T"
+  by (dp_match induct: su\<^sub>T.induct simp: su.simps simp\<^sub>T: su\<^sub>T.simps)
+
+end
+end
